Solidity/Kernel/Erase.lean
@@ -40,8 +40,8 @@ def Loc.erase {C : Contract} {Γ : Ctx} {T : Ty} : Loc C Γ T → WrappedExpr
 def Val.erase {C : Contract} {Γ : Ctx} {p : PrimTy} : Val C Γ p → WrappedExpr
   | .simple s => s.erase
   | .read l => l.erase
-  | .binop op _ a b => .mkBinop op a.erase b.erase
-  | .unop op _ a => .mkUnop op a.erase
+  | .binop op _ _ a b => .mkBinop op a.erase b.erase
+  | .unop op _ _ a => .mkUnop op a.erase
 
 end
 
@@ -74,10 +74,10 @@ theorem Val.erase_ty {C : Contract} {Γ : Ctx} {p : PrimTy} :
     (v : Val C Γ p) → v.erase.ty = .prim p
   | .simple s => s.erase_ty
   | .read l => l.erase_ty
-  | .binop op _ a _ => by
-      simp only [Val.erase, Typed.WrappedExpr.ty, a.erase_ty, BinOp.retTy_prim]
-  | .unop op _ a => by
-      simp only [Val.erase, Typed.WrappedExpr.ty, a.erase_ty, UnOp.retTy_prim]
+  | .binop op _ hq a _ => by
+      simp only [Val.erase, Typed.WrappedExpr.ty, a.erase_ty, BinOp.retTy_prim, hq]
+  | .unop op _ hq a => by
+      simp only [Val.erase, Typed.WrappedExpr.ty, a.erase_ty, UnOp.retTy_prim, hq]
 
 end
 
@@ -131,8 +131,8 @@ theorem Val.erase_wt {C : Contract} {Γ : Ctx} {p : PrimTy} :
     (v : Val C Γ p) → wtExpr Γ C.layout v.erase = true
   | .simple s => s.erase_wt
   | .read l => l.erase_wt
-  | .binop _ _ a b => by simp [Val.erase, wtExpr, a.erase_wt, b.erase_wt]
-  | .unop _ _ a => by simp [Val.erase, wtExpr, a.erase_wt]
+  | .binop _ _ _ a b => by simp [Val.erase, wtExpr, a.erase_wt, b.erase_wt]
+  | .unop _ _ _ a => by simp [Val.erase, wtExpr, a.erase_wt]
 
 end
 
